Unfix f in flat combiner; Unifies atomic_triple

atomic_sync.v
@@ -13,9 +13,7 @@ Instance subG_syncΣ {Σ} : subG syncΣ Σ → syncG Σ.
 Proof. by intros ?%subG_inG. Qed.
 
 Section atomic_sync.
-  Context `{!heapG Σ, !lockG Σ, !inG Σ (prodR fracR (dec_agreeR val))} (N : namespace).
-
-  Definition A := val. (* FIXME: can't use a general A instead of val *)
+  Context `{EqDecision A, !heapG Σ, !lockG Σ, !inG Σ (prodR fracR (dec_agreeR A))} (N : namespace).
 
   Definition gHalf (γ: gname) g : iProp Σ := own γ ((1/2)%Qp, DecAgree g).
 
@@ -24,15 +22,16 @@ Section atomic_sync.
              (β: val → A → A → val → iProp Σ)
              (Ei Eo: coPset)
              (f x: val) γ : iProp Σ :=
-    (∀ P Q, (∀ g, (P x ={Eo, Ei}=> gHalf γ g ★ □ α x) ★
-                  (gHalf γ g ★ □ α x ={Ei, Eo}=> P x) ★
-                  (∀ g' r, gHalf γ g' ★ β x g g' r ={Ei, Eo}=> Q x r))
-            -★ {{ P x }} f x {{ v, Q x v }})%I.
-
-  Definition sync (syncer: val) : val :=
+    (∀ P Q, atomic_triple_base A (fun g => gHalf γ g ★ □ α x)
+                                 (fun g v => ∃ g':A, gHalf γ g' ★ β x g g' v)
+                                 Ei Eo
+                                (f x) (P x) (fun _ => Q x))%I.
+       
+  Definition sync (mk_syncer: val) : val :=
     λ: "f_cons" "f_seq",
-        let: "l"  := "f_cons" #() in
-        syncer ("f_seq" "l").
+       let: "l" := "f_cons" #() in
+       let: "s" := mk_syncer #() in
+       "s" ("f_seq" "l").
 
   Definition seq_spec (f: val) (ϕ: val → A → iProp Σ) α β (E: coPset) :=
       ∀ (Φ: val → iProp Σ) (l: val),
@@ -48,55 +47,66 @@ Section atomic_sync.
         ⊢ WP f #() {{ Φ }}.
 
   Definition synced R (f' f: val) :=
-    (∀ P Q (x: val), ({{ R ★ P x }} f x {{ v, R ★ Q x v }}) → ({{ P x }} f' x {{ v, Q x v }}))%I.
+    (□ ∀ P Q (x: val), ({{ R ★ P x }} f x {{ v, R ★ Q x v }}) → ({{ P x }} f' x {{ v, Q x v }}))%I.
 
-  Definition mk_sync_spec (syncer: val) :=
-    ∀ f R (Φ: val → iProp Σ),
-      heapN ⊥ N → 
-      heap_ctx ★ R ★ (∀ f', □ synced R f' f -★ Φ f') ⊢ WP syncer f {{ Φ }}.
+  Definition is_syncer (R: iProp Σ) (s: val) :=
+    (∀ (f : val), WP s f {{ f', synced R f' f }})%I.
+
+  Definition mk_syncer_spec (mk_syncer: val) :=
+    ∀ (R: iProp Σ) (Φ: val -> iProp Σ),
+      heapN ⊥ N →
+      heap_ctx ★ R ★ (∀ s, □ (is_syncer R s) -★ Φ s) ⊢ WP mk_syncer #() {{ Φ }}.
   
-  Lemma atomic_spec (syncer f_cons f_seq: val) (ϕ: val → A → iProp Σ) α β Ei:
+  Lemma atomic_spec (mk_syncer f_cons f_seq: val) (ϕ: val → A → iProp Σ) α β Ei:
       ∀ (g0: A),
         heapN ⊥ N → seq_spec f_seq ϕ α β ⊤ → cons_spec f_cons g0 ϕ →
-        mk_sync_spec syncer →
+        mk_syncer_spec mk_syncer →
         heap_ctx
-        ⊢ WP (sync syncer) f_cons f_seq {{ f, ∃ γ, gHalf γ g0 ★ ∀ x, □ atomic_triple' α β Ei ⊤ f x γ  }}.
+        ⊢ WP (sync mk_syncer) f_cons f_seq {{ f, ∃ γ, gHalf γ g0 ★ ∀ x, □ atomic_triple' α β Ei ⊤ f x γ  }}.
   Proof.
     iIntros (g0 HN Hseq Hcons Hsync) "#Hh". repeat wp_let.
     wp_bind (f_cons _). iApply Hcons=>//. iFrame "Hh".
     iIntros (l γ) "Hϕ HFull HFrag".
-    wp_let. wp_bind (f_seq _)%E.
-    iApply wp_wand_r. iSplitR; first by iApply (Hseq with "[]")=>//.
-    iIntros (f Hf). iApply (Hsync f (∃ g: A, ϕ l g ★ gHalf γ g)%I)=>//.
-    iFrame "#". iSplitL "HFull Hϕ".
+    wp_let. wp_bind (mk_syncer _).
+    iApply (Hsync (∃ g: A, ϕ l g ★ gHalf γ g)%I)=>//. iFrame "Hh".
+    iSplitL "HFull Hϕ".
     { iExists g0. by iFrame. }
-    iIntros (f') "#Hflatten".
+    iIntros (s) "#Hsyncer".
+    wp_let. wp_bind (f_seq _). iApply wp_wand_r.
+    iSplitR; first by iApply (Hseq with "[]")=>//.
+    iIntros (f) "%".
+    iApply wp_wand_r.
+    iSplitR; first iApply "Hsyncer".
+    iIntros (f') "#Hsynced".
     iExists γ. iFrame.
     iIntros (x). iAlways.
     rewrite /atomic_triple'.
     iIntros (P Q) "#Hvss".
     rewrite /synced.
-    iSpecialize ("Hflatten" $! P Q).
-    iApply ("Hflatten" with "[]").
-    iAlways. iIntros "[HR HP]". iDestruct "HR" as (g) "[Hϕ HgFull]".
-    (* we should view shift at this point *)
-    iDestruct ("Hvss" $! g) as "[Hvs1 [Hvs2 Hvs3]]".
-    iApply pvs_wp.
-    iVs ("Hvs1" with "HP") as "[HgFrag #Hα]".
-    iVs ("Hvs2" with "[HgFrag]") as "HP"; first by iFrame.
-    iVsIntro. iApply Hf=>//.
-    iFrame "Hh Hϕ". iSplitR; first done. iIntros (ret g') "Hϕ' Hβ".
-    iVs ("Hvs1" with "HP") as "[HgFrag _]".
-    iCombine "HgFull" "HgFrag" as "Hg".
-    rewrite /gHalf.
-    iAssert (|=r=> own γ (((1 / 2)%Qp, DecAgree g') ⋅ ((1 / 2)%Qp, DecAgree g')))%I with "[Hg]" as "Hupd".
-    { iApply (own_update); last by iAssumption. apply pair_l_frac_update. }
-    iVs "Hupd" as "[HgFull HgFrag]".
-    iVs ("Hvs3" $! g' ret with "[HgFrag Hβ]"); first by iFrame.
-    iVsIntro.
-    iSplitL "HgFull Hϕ'".
-    - iExists g'. by iFrame.
-    - done.
+    iSpecialize ("Hsynced" $! P Q x). 
+    iIntros "!# HP". iApply wp_wand_r. iSplitL "HP".
+    - iApply ("Hsynced" with "[]")=>//.
+      iAlways. iIntros "[HR HP]". iDestruct "HR" as (g) "[Hϕ Hg1]".
+      (* we should view shift at this point *) 
+      iDestruct ("Hvss" with "HP") as "Hvss'". iApply pvs_wp.
+      iVs "Hvss'". iDestruct "Hvss'" as (?) "[[Hg2 #Hα] [Hvs1 _]]".
+      iVs ("Hvs1" with "[Hg2]") as "HP"; first by iFrame.
+      iVsIntro. iApply H=>//.
+      iFrame "Hh Hϕ". iSplitR; first done. iIntros (ret g') "Hϕ' Hβ".
+      iVs ("Hvss" with "HP") as (g'') "[[Hg'' _] [_ Hvs2]]".
+      iSpecialize ("Hvs2" $! ret).
+      iDestruct (m_frag_agree' with "[Hg'' Hg1]") as "[Hg %]"; first iFrame. subst.
+      rewrite Qp_div_2.
+      iAssert (|=r=> own γ (((1 / 2)%Qp, DecAgree g') ⋅ ((1 / 2)%Qp, DecAgree g')))%I
+              with "[Hg]" as "==>[Hg1 Hg2]".
+      { iApply own_update; last by iAssumption.
+        apply cmra_update_exclusive. by rewrite pair_op dec_agree_idemp. }        
+      iVs ("Hvs2" with "[Hg1 Hβ]").
+      { iExists g'. iFrame. }
+      iVsIntro. iSplitL "Hg2 Hϕ'".
+      * iExists g'. by iFrame.
+      * done.
+    - iIntros (?) "?". by iExists g0.
   Qed.
-  
+
 End atomic_sync.
